11FlatMemory/FlatMemory.thy
@@ -5,16 +5,16 @@ begin
 text \<open>The chained memory stage is quite low-level, but it still possesses some structured data: 
 pairs in the stack and the environment heap, and tagged closure-values in the value heap. We now 
 reduce all of these to contiguous series of numbers. The stack pairs are just listed, first 
-component first; the environment pairs are listed, first the environment frame in reverse order and 
-then the cons-pointer. The closures are flattened to sequences of data: a \<open>Const\<^sub>v n\<close> value becomes 
-\<open>[n, 0]\<close>; a \<open>Lam\<^sub>v p\<^sub>\<Delta> p\<^sub>\<C> n\<close> becomes \<open>[p\<^sub>\<Delta>, p\<^sub>\<C>]\<close>. (The padding 0 on the numerical values is just to 
-keep all values the same size, greatly easing some of the proofs.) We also tag the code and 
-environment pointers because we need to recognize them later, when we move to assembly code and 
-alter all the codeblock addresses; besides that, in losing the value constructors and the implicit 
-tag that goes with that, we have now discarded our last scrap of source-level type-safety. The 
-\<open>ev\<^sub>f_apply\<close> and \<open>ev\<^sub>f_jump\<close> operations assume they've been given a function-closure, and check that 
-they have environment and code pointers, but the memory itself no longer records as such that there 
-is a function stored there.\<close>
+component first; the environment pairs are listed, first the cons-pointer and then the environment 
+frame. The closures are flattened to sequences of data: a \<open>Const\<^sub>v n\<close> value becomes \<open>[n, 0]\<close>; a 
+\<open>Lam\<^sub>v p\<^sub>\<Delta> p\<^sub>\<C> n\<close> becomes \<open>[p\<^sub>\<Delta>, p\<^sub>\<C>]\<close>. (The padding 0 on the numerical values is just to keep all values 
+the same size, greatly easing some of the proofs.) We also tag the code and environment pointers 
+because we need to recognize them later, when we move to assembly code and alter all the codeblock 
+addresses; besides that, in losing the value constructors and the implicit tag that goes with that, 
+we have now discarded our last scrap of source-level type-safety. The \<open>ev\<^sub>f_apply\<close> and \<open>ev\<^sub>f_jump\<close> 
+operations assume they've been given a function-closure, and check that they have environment and 
+code pointers, but the memory itself no longer records as such that there is a function stored 
+there.\<close>
 
 datatype state\<^sub>f = 
   S\<^sub>f "(pointer_tag \<times> nat) heap" "ptr heap" "ptr list" "nat list"
@@ -27,19 +27,21 @@ fun flat_lookup :: "ptr heap \<Rightarrow> ptr \<Rightarrow> nat \<Rightarrow> n
     if even p then flat_lookup h (hlookup h (Suc p)) x y else None)"
 
 inductive eval\<^sub>f :: "code\<^sub>b list \<Rightarrow> state\<^sub>f \<Rightarrow> state\<^sub>f \<Rightarrow> bool" (infix "\<tturnstile> _ \<leadsto>\<^sub>f" 50) where
-  ev\<^sub>f_lookup [simp]: "lookup \<C> p\<^sub>\<C> = Some (Lookup\<^sub>b x y z) \<Longrightarrow> flat_lookup \<Delta> p\<^sub>\<Delta> x = Some v \<Longrightarrow> 
+  ev\<^sub>f_lookup [simp]: "lookup \<C> p\<^sub>\<C> = Some (Lookup\<^sub>b x y) \<Longrightarrow> flat_lookup \<Delta> p\<^sub>\<Delta> x y = Some v \<Longrightarrow> 
     \<C> \<tturnstile> S\<^sub>f h \<Delta> \<V> (Suc p\<^sub>\<C> # p\<^sub>\<Delta> # s) \<leadsto>\<^sub>f S\<^sub>f h \<Delta> (v # \<V>) (p\<^sub>\<C> # p\<^sub>\<Delta> # s)"
 | ev\<^sub>f_pushcon [simp]: "lookup \<C> p\<^sub>\<C> = Some (PushCon\<^sub>b n) \<Longrightarrow> 
     halloc_list h [(PConst, n), (PConst, 0)] = (h', v) \<Longrightarrow>
       \<C> \<tturnstile> S\<^sub>f h \<Delta> \<V> (Suc p\<^sub>\<C> # p\<^sub>\<Delta> # s) \<leadsto>\<^sub>f S\<^sub>f h' \<Delta> (v # \<V>) (p\<^sub>\<C> # p\<^sub>\<Delta> # s)"
-| ev\<^sub>f_pushlam [simp]: "lookup \<C> p\<^sub>\<C> = Some (PushLam\<^sub>b p\<^sub>\<C>' n) \<Longrightarrow> 
+| ev\<^sub>f_pushlam [simp]: "lookup \<C> p\<^sub>\<C> = Some (PushLam\<^sub>b p\<^sub>\<C>') \<Longrightarrow> 
     halloc_list h [(PEnv, p\<^sub>\<Delta>), (PCode, p\<^sub>\<C>')] = (h', v) \<Longrightarrow> 
       \<C> \<tturnstile> S\<^sub>f h \<Delta> \<V> (Suc p\<^sub>\<C> # p\<^sub>\<Delta> # s) \<leadsto>\<^sub>f S\<^sub>f h' \<Delta> (v # \<V>) (p\<^sub>\<C> # p\<^sub>\<Delta> # s)"
+| ev\<^sub>f_alloc [simp]: "lookup \<C> p\<^sub>\<C> = Some (Alloc\<^sub>b n) \<Longrightarrow> 
+    \<C> \<tturnstile> S\<^sub>f h \<Delta> \<V> (Suc p\<^sub>\<C> # p\<^sub>\<Delta> # s) \<leadsto>\<^sub>f S\<^sub>f h \<Delta> \<V> (p\<^sub>\<C> # (p\<^sub>\<Delta> + n) # s)"
 | ev\<^sub>f_apply [simp]: "lookup \<C> p\<^sub>\<C> = Some Apply\<^sub>b \<Longrightarrow> hlookup h v\<^sub>2 = (PEnv, p\<^sub>\<Delta>') \<Longrightarrow> 
     hlookup h (Suc v\<^sub>2) = (PCode, p\<^sub>\<C>') \<Longrightarrow> halloc_list \<Delta> [v\<^sub>1, p\<^sub>\<Delta>'] = (\<Delta>', p\<^sub>\<Delta>'') \<Longrightarrow> 
       \<C> \<tturnstile> S\<^sub>f h \<Delta> (v\<^sub>1 # v\<^sub>2 # \<V>) (Suc p\<^sub>\<C> # p\<^sub>\<Delta> # s) \<leadsto>\<^sub>f S\<^sub>f h \<Delta>' \<V> (p\<^sub>\<C>' # Suc (Suc p\<^sub>\<Delta>'') # p\<^sub>\<C> # p\<^sub>\<Delta> # s)"
-| ev\<^sub>f_pushenv [simp]: "lookup \<C> p\<^sub>\<C> = Some PushEnv\<^sub>b \<Longrightarrow> halloc_list \<Delta> [v, p\<^sub>\<Delta>] = (\<Delta>', p\<^sub>\<Delta>') \<Longrightarrow> 
-    \<C> \<tturnstile> S\<^sub>f h \<Delta> (v # \<V>) (Suc p\<^sub>\<C> # p\<^sub>\<Delta> # s) \<leadsto>\<^sub>f S\<^sub>f h \<Delta>' \<V> (p\<^sub>\<C> # Suc (Suc p\<^sub>\<Delta>') # s)"
+| ev\<^sub>f_pushenv [simp]: "lookup \<C> p\<^sub>\<C> = Some (PushEnv\<^sub>b n) \<Longrightarrow> 
+    \<C> \<tturnstile> S\<^sub>f h \<Delta> (v # \<V>) (Suc p\<^sub>\<C> # p\<^sub>\<Delta> # s) \<leadsto>\<^sub>f S\<^sub>f h (hupdate \<Delta> (p\<^sub>\<Delta> + n) v) \<V> (p\<^sub>\<C> # p\<^sub>\<Delta> # s)"
 | ev\<^sub>f_return [simp]: "lookup \<C> p\<^sub>\<C> = Some Return\<^sub>b \<Longrightarrow> 
     \<C> \<tturnstile> S\<^sub>f h \<Delta> \<V> (Suc p\<^sub>\<C> # p\<^sub>\<Delta> # s) \<leadsto>\<^sub>f S\<^sub>f h \<Delta> \<V> s"
 | ev\<^sub>f_jump [simp]: "lookup \<C> p\<^sub>\<C> = Some Jump\<^sub>b \<Longrightarrow> hlookup h v\<^sub>2 = (PEnv, p\<^sub>\<Delta>') \<Longrightarrow> 
@@ -57,11 +59,14 @@ next
   case ev\<^sub>f_pushlam
   from ev\<^sub>f_pushlam(3, 1, 2) show ?case by (induction rule: eval\<^sub>f.cases) simp_all  
 next
+  case ev\<^sub>f_alloc
+  from ev\<^sub>f_alloc(2, 1) show ?case by (induction rule: eval\<^sub>f.cases) simp_all  
+next
   case ev\<^sub>f_apply
   from ev\<^sub>f_apply(5, 1, 2, 3, 4) show ?case by (induction rule: eval\<^sub>f.cases) simp_all  
 next
   case ev\<^sub>f_pushenv
-  from ev\<^sub>f_pushenv(3, 1, 2) show ?case by (induction rule: eval\<^sub>f.cases) simp_all  
+  from ev\<^sub>f_pushenv(2, 1) show ?case by (induction rule: eval\<^sub>f.cases) simp_all  
 next
   case ev\<^sub>f_return
   from ev\<^sub>f_return(2, 1) show ?case by (induction rule: eval\<^sub>f.cases) simp_all 
